ValidAddresses.v
@@ -5,283 +5,132 @@ From Coq Require Classical_Prop.
 From Elo Require Import Util.
 From Elo Require Import Array.
 From Elo Require Import Core.
+From Elo Require Import HasAddress.
 
-(* -------------------------------------------------------------------------- *)
-(* has-address                                                                *)
-(* -------------------------------------------------------------------------- *)
 
-Inductive HasAddress (ad : addr) : tm -> Prop :=
-  | hasad_ref : forall T,
-    HasAddress ad <{ &ad :: T }>
-
-  | hasad_new : forall t T,
-    HasAddress ad t ->
-    HasAddress ad <{ new T t }>
-
-  | hasad_load : forall t,
-    HasAddress ad t ->
-    HasAddress ad <{ *t }>
-
-  | hasad_asg1 : forall t1 t2,
-    HasAddress ad t1 ->
-    HasAddress ad <{ t1 = t2 }>
-
-  | hasad_asg2 : forall t1 t2,
-    HasAddress ad t2 ->
-    HasAddress ad <{ t1 = t2 }>
-
-  | hasad_fun : forall t x Tx,
-    HasAddress ad t ->
-    HasAddress ad <{ fn x Tx --> t }>
-
-  | hasad_call1 : forall t1 t2,
-    HasAddress ad t1 ->
-    HasAddress ad <{ call t1 t2 }>
-
-  | hasad_call2 : forall t1 t2,
-    HasAddress ad t2 ->
-    HasAddress ad <{ call t1 t2 }>
-
-  | hasad_seq1 : forall t1 t2,
-    HasAddress ad t1 ->
-    HasAddress ad <{ t1; t2 }>
-
-  | hasad_seq2 : forall t1 t2,
-    HasAddress ad t2 ->
-    HasAddress ad <{ t1; t2 }>
-
-  | hasad_spawn : forall t,
-    HasAddress ad t ->
-    HasAddress ad <{ spawn t }>
-  .
-
-Lemma hasad_dec : forall ad t,
-  Decidable.decidable (HasAddress ad t).
-Proof. intros. eauto using classic_decidable. Qed.
-
-(* -------------------------------------------------------------------------- *)
-(* inversion-ha                                                               *)
-(* -------------------------------------------------------------------------- *)
-
-Ltac inversion_ha :=
-  match goal with
-  | H : HasAddress _ <{ unit         }> |- _ => inversion H
-  | H : HasAddress _ <{ N _          }> |- _ => inversion H
-  | H : HasAddress _ <{ & _ :: _     }> |- _ => inversion H; subst
-  | H : HasAddress _ <{ new _ _      }> |- _ => inversion H; subst
-  | H : HasAddress _ <{ * _          }> |- _ => inversion H; subst
-  | H : HasAddress _ <{ _ = _        }> |- _ => inversion H; subst
-  | H : HasAddress _ <{ var _        }> |- _ => inversion H
-  | H : HasAddress _ <{ fn _ _ --> _ }> |- _ => inversion H; subst
-  | H : HasAddress _ <{ call _ _     }> |- _ => inversion H; subst
-  | H : HasAddress _ <{ _ ; _        }> |- _ => inversion H; subst
-  | H : HasAddress _ <{ spawn _      }> |- _ => inversion H; subst
-  end.
-
-(* -------------------------------------------------------------------------- *)
-(* inversion-nha                                                              *)
-(* -------------------------------------------------------------------------- *)
-
-Local Ltac solve_inv_nha1 :=
-  intros; intros ?; eauto using HasAddress.
-
-Local Ltac solve_inv_nha2 :=
-  intros * F; eapply Classical_Prop.not_or_and;
-  intros [? | ?]; eapply F; eauto using HasAddress.
-
-Local Lemma inv_nha_ref : forall ad ad' T,
-  ~ HasAddress ad <{ &ad' :: T}> ->
-  ad <> ad'.
-Proof. intros. intros ?. subst. eauto using HasAddress. Qed.
-
-Local Lemma inv_nha_new : forall ad t T,
-  ~ HasAddress ad <{ new T t }> ->
-  ~ HasAddress ad t.
-Proof. solve_inv_nha1. Qed.
-
-Local Lemma inv_nha_load : forall ad t,
-  ~ HasAddress ad <{ *t }> ->
-  ~ HasAddress ad t.
-Proof. solve_inv_nha1. Qed.
-
-Local Lemma inv_nha_asg : forall ad t1 t2,
-  ~ HasAddress ad <{ t1 = t2 }> ->
-  (~ HasAddress ad t1) /\ (~ HasAddress ad t2).
-Proof. solve_inv_nha2. Qed.
-
-Local Lemma inv_nha_fun : forall ad t x Tx,
-  ~ HasAddress ad <{ fn x Tx --> t }> ->
-  ~ HasAddress ad t.
-Proof. solve_inv_nha1. Qed.
-
-Local Lemma inv_nha_call : forall ad t1 t2,
-  ~ HasAddress ad <{ call t1 t2 }> ->
-  (~ HasAddress ad t1) /\ (~ HasAddress ad t2).
-Proof. solve_inv_nha2. Qed.
-
-Local Lemma inv_nha_seq : forall ad t1 t2,
-  ~ HasAddress ad <{ t1; t2 }> ->
-  (~ HasAddress ad t1) /\ (~ HasAddress ad t2).
-Proof. solve_inv_nha2. Qed.
-
-Local Lemma inv_nha_spawn : forall ad t,
-  ~ HasAddress ad <{ spawn t }> ->
-  ~ HasAddress ad t.
-Proof. solve_inv_nha1. Qed.
-
-Ltac inversion_nha :=
-  match goal with
-  | H : ~ HasAddress _ <{ & _ :: _ }> |- _ => eapply inv_nha_ref   in H
-  | H : ~ HasAddress _ <{ new _ _  }> |- _ => eapply inv_nha_new   in H
-  | H : ~ HasAddress _ <{ * _      }> |- _ => eapply inv_nha_load  in H
-  | H : ~ HasAddress _ <{ _ = _    }> |- _ => eapply inv_nha_asg   in H as [? ?]
-  | H : ~ HasAddress _ <{ fn _ _ --> _ }> |- _ => eapply inv_nha_fun in H
-  | H : ~ HasAddress _ <{ call _ _ }> |- _ => eapply inv_nha_call  in H as [? ?]
-  | H : ~ HasAddress _ <{ _ ; _    }> |- _ => eapply inv_nha_seq   in H as [? ?]
-  | H : ~ HasAddress _ <{ spawn _  }> |- _ => eapply inv_nha_spawn in H
-  end.
-
-(* ------------------------------------------------------------------------- *)
-(* has-address helpers                                                       *)
-(* ------------------------------------------------------------------------- *)
-
-Lemma step_write_hasad1 : forall t t' ad v V,
-  t --[EF_Write ad v V]--> t' ->
-  HasAddress ad t.
-Proof. intros. induction_step; eauto using HasAddress. Qed.
-
-Lemma step_write_hasad2 : forall t t' ad ad' v V,
-  HasAddress ad v ->
-  t --[EF_Write ad' v V]--> t' ->
-  HasAddress ad t.
-Proof. intros. induction_step; eauto using HasAddress. Qed.
-
-(* -------------------------------------------------------------------------- *)
-(* valid-addresses                                                            *)
-(* -------------------------------------------------------------------------- *)
-
+(* The addresses of a term are valid if they
+are smaller than the length of the memory. *)
 Definition valid_addresses (m : mem) (t : tm) :=
-  forall ad, HasAddress ad t -> ad < length m.
+  forall ad, HasAddress ad t -> ad < #m.
 
-Local Ltac solve_con_va := 
+(* ------------------------------------------------------------------------- *)
+(* constructors                                                              *)
+(* ------------------------------------------------------------------------- *)
+
+Local Ltac solve_va_constructor := 
   intros; intros ? ?; inversion_ha; eauto.
 
-Local Lemma va_unit: forall m,
+Local Lemma va_unit : forall m,
   valid_addresses m <{ unit }>.
-Proof. solve_con_va. Qed.
+Proof. solve_va_constructor. Qed.
 
-Local Lemma va_num: forall m n,
-  valid_addresses m <{ N n }>.
-Proof. solve_con_va. Qed.
-
-Local Lemma va_new: forall m t T,
+Local Lemma va_new : forall m t T,
   valid_addresses m t ->
   valid_addresses m <{ new T t }>.
-Proof. solve_con_va. Qed.
+Proof. solve_va_constructor. Qed.
 
 Local Lemma va_load : forall m t,
   valid_addresses m t ->
   valid_addresses m <{ *t }>.
-Proof. solve_con_va. Qed.
+Proof. solve_va_constructor. Qed.
 
 Local Lemma va_asg : forall m t1 t2,
   valid_addresses m t1 ->
   valid_addresses m t2 ->
   valid_addresses m <{ t1 = t2 }>.
-Proof. solve_con_va. Qed.
+Proof. solve_va_constructor. Qed.
 
 Local Lemma va_fun : forall m x Tx t,
   valid_addresses m t ->
   valid_addresses m <{ fn x Tx --> t }>.
-Proof. solve_con_va. Qed.
+Proof. solve_va_constructor. Qed.
 
 Local Lemma va_call : forall m t1 t2,
   valid_addresses m t1 ->
   valid_addresses m t2 ->
   valid_addresses m <{ call t1 t2 }>.
-Proof. solve_con_va. Qed.
+Proof. solve_va_constructor. Qed.
 
 Local Lemma va_seq : forall m t1 t2,
   valid_addresses m t1 ->
   valid_addresses m t2 ->
   valid_addresses m <{ t1; t2 }>.
-Proof. solve_con_va. Qed.
+Proof. solve_va_constructor. Qed.
 
 Local Lemma va_spawn : forall m t,
   valid_addresses m t ->
   valid_addresses m <{ spawn t }>.
-Proof. solve_con_va. Qed.
+Proof. solve_va_constructor. Qed.
 
-(* -------------------------------------------------------------------------- *)
-(* inversion-va                                                               *)
-(* -------------------------------------------------------------------------- *)
+(* ------------------------------------------------------------------------- *)
+(* inversion                                                                 *)
+(* ------------------------------------------------------------------------- *)
 
-Local Ltac solve_inv_va := 
+Local Ltac solve_va_inversion := 
   intros; unfold valid_addresses in *; try split; eauto using HasAddress.
 
 Local Lemma inv_va_ref : forall m ad T,
   valid_addresses m <{ &ad :: T }> ->
   ad < length m.
-Proof. intros. unfold valid_addresses in *. eauto using HasAddress. Qed.
+Proof. solve_va_inversion. Qed.
 
 Local Lemma inv_va_new : forall m t T,
   valid_addresses m <{ new T t }> ->
   valid_addresses m t.
-Proof. solve_inv_va. Qed.
+Proof. solve_va_inversion. Qed.
 
 Local Lemma inv_va_load : forall m t,
   valid_addresses m <{ *t }> ->
   valid_addresses m t.
-Proof. solve_inv_va. Qed.
+Proof. solve_va_inversion. Qed.
 
 Local Lemma inv_va_asg : forall m t1 t2,
   valid_addresses m <{ t1 = t2 }> ->
   valid_addresses m t1 /\ valid_addresses m t2.
-Proof. solve_inv_va. Qed.
+Proof. solve_va_inversion. Qed.
 
 Local Lemma inv_va_fun : forall m x Tx t,
   valid_addresses m <{ fn x Tx --> t }> ->
   valid_addresses m t.
-Proof. solve_inv_va. Qed.
+Proof. solve_va_inversion. Qed.
 
 Local Lemma inv_va_call : forall m t1 t2,
   valid_addresses m <{ call t1 t2 }> ->
   valid_addresses m t1 /\ valid_addresses m t2.
-Proof. solve_inv_va. Qed.
+Proof. solve_va_inversion. Qed.
 
 Local Lemma inv_va_seq : forall m t1 t2,
   valid_addresses m <{ t1; t2 }> ->
   valid_addresses m t1 /\ valid_addresses m t2.
-Proof. solve_inv_va. Qed.
+Proof. solve_va_inversion. Qed.
 
 Local Lemma inv_va_spawn : forall m t,
   valid_addresses m <{ spawn t }> ->
   valid_addresses m t.
-Proof. solve_inv_va. Qed.
+Proof. solve_va_inversion. Qed.
 
 Ltac inversion_va :=
   match goal with
-  | H: valid_addresses _ <{ & ?ad :: _ }> |- _ => eapply inv_va_ref in H as ?
-  | H: valid_addresses _ <{ new _ _ }> |- _ => eapply inv_va_new  in H
-  | H: valid_addresses _ <{ * _     }> |- _ => eapply inv_va_load in H
-  | H: valid_addresses _ <{ _ = _   }> |- _ => eapply inv_va_asg  in H as [? ?]
+  | H: valid_addresses _ <{ & _ :: _ }> |- _ => eapply inv_va_ref  in H as ?
+  | H: valid_addresses _ <{ new _ _  }> |- _ => eapply inv_va_new  in H
+  | H: valid_addresses _ <{ * _      }> |- _ => eapply inv_va_load in H
+  | H: valid_addresses _ <{ _ = _    }> |- _ => eapply inv_va_asg  in H as [? ?]
   | H: valid_addresses _ <{ fn _ _ --> _ }> |- _ => eapply inv_va_fun in H
   | H: valid_addresses _ <{ call _ _ }> |- _ => eapply inv_va_call in H as [? ?]
   | H: valid_addresses _ <{ _ ; _    }> |- _ => eapply inv_va_seq  in H as [? ?]
   | H: valid_addresses _ <{ spawn _  }> |- _ => eapply inv_va_spawn in H
   end.
 
-(* -------------------------------------------------------------------------- *)
-(* va-preservation helpers                                                    *)
-(* -------------------------------------------------------------------------- *)
+(* ------------------------------------------------------------------------- *)
+(* preservation helpers                                                      *)
+(* ------------------------------------------------------------------------- *)
 
 Local Lemma va_subst : forall m t tx x,
   valid_addresses m t ->
   valid_addresses m tx ->
   valid_addresses m ([x := tx] t).
 Proof.
-  intros. induction t;
-  try inversion_va; simpl;
+  intros. induction t; try inversion_va; simpl;
   eauto using va_new, va_load, va_asg, va_call, va_seq, va_fun, va_spawn;
   destruct String.string_dec; subst; trivial;
   intros ? ?; inversion_ha; unfold valid_addresses in *; eauto.
@@ -291,8 +140,8 @@ Local Lemma mem_add_va : forall m t v,
   valid_addresses m t ->
   valid_addresses (m +++ v) t.
 Proof.
-  intros * ? ? Hha. induction Hha; inversion_va; eauto.
-  rewrite add_increments_length. lia.
+  intros * ? ? Hha. rewrite add_increments_length.
+  induction Hha; inversion_va; eauto.
 Qed.
 
 Local Lemma mem_set_va : forall m t ad v V,
@@ -304,9 +153,18 @@ Proof.
   induction Hha; inversion_va; eauto.
 Qed.
 
-(* -------------------------------------------------------------------------- *)
-(* va-preservation                                                            *)
-(* -------------------------------------------------------------------------- *)
+Local Lemma spawn_block_va : forall m t t' block,
+  valid_addresses m t ->
+  t --[EF_Spawn block]--> t' ->
+  valid_addresses m block.
+Proof.
+  intros. induction_step; inversion_va; eauto.
+Qed.
+
+
+(* ------------------------------------------------------------------------- *)
+(* term preservation                                                         *)
+(* ------------------------------------------------------------------------- *)
 
 Local Lemma step_none_va_preservation : forall m t t',
   valid_addresses m t ->
@@ -324,7 +182,7 @@ Local Lemma step_alloc_va_preservation : forall m t t' v V,
   valid_addresses (m +++ (v, V)) t'.
 Proof.
   intros. induction_step; inversion_va;
-  eauto using va_new, va_load, va_asg, va_call, va_seq, mem_add_va.
+  eauto using mem_add_va, va_new, va_load, va_asg, va_call, va_seq.
   intros ? ?. inversion_ha. rewrite add_increments_length. lia.
 Qed.
 
@@ -345,12 +203,12 @@ Local Lemma step_write_va_preservation : forall m t t' ad v V,
 Proof.
   intros. assert (valid_addresses m v) by shelve.
   induction_step; inversion_va;
-  eauto using va_unit, va_new, va_load, va_asg, va_call, va_seq, mem_set_va.
+  eauto using mem_set_va, va_unit, va_new, va_load, va_asg, va_call, va_seq.
   Unshelve. intros ? ?. induction_step; inversion_va; eauto.
 Qed.
 
 Local Corollary mstep_va_preservation : forall m m' t t' eff,
-  forall_memory_terms m (valid_addresses m) ->
+  forall_memory m (valid_addresses m) ->
   valid_addresses m t ->
   m / t ==[eff]==> m' / t' ->
   valid_addresses m' t'.
@@ -371,37 +229,31 @@ Proof.
   eauto using va_unit, va_new, va_load, va_asg, va_call, va_seq.
 Qed.
 
-(* -------------------------------------------------------------------------- *)
-(* mem-va-preservation                                                        *)
-(* -------------------------------------------------------------------------- *)
-
-Local Lemma hasad_alloc_term : forall t t' ad ad' v V,
-  HasAddress ad v ->
-  t --[EF_Alloc ad' v V]--> t' ->
-  HasAddress ad t.
-Proof. intros. induction_step; eauto using HasAddress. Qed.
+(* ------------------------------------------------------------------------- *)
+(* memory preservation                                                       *)
+(* ------------------------------------------------------------------------- *)
 
 Local Lemma step_alloc_mem_va_preservation : forall m t t' v V,
   valid_addresses m t ->
-  forall_memory_terms m (valid_addresses m) ->
+  forall_memory m (valid_addresses m) ->
   t --[EF_Alloc (length m) v V]--> t' ->
-  forall_memory_terms  (m +++ (v, V)) (valid_addresses (m +++ (v, V))).
+  forall_memory  (m +++ (v, V)) (valid_addresses (m +++ (v, V))).
 Proof.
-  intros. intros ad. decompose sum (lt_eq_lt_dec ad (length m)); subst;
-  simpl_array; intros ? ?; rewrite add_increments_length;
-  unfold valid_addresses in *; eauto using hasad_alloc_term, Nat.lt_lt_succ_r.
+  intros. intros ad.
+  decompose sum (lt_eq_lt_dec ad (length m)); subst; simpl_array;
+  intros ? ?; rewrite add_increments_length;
+  unfold valid_addresses in *; eauto using step_alloc_hasad, Nat.lt_lt_succ_r.
   simpl in *. inversion_ha.
 Qed.
 
 Local Lemma step_write_mem_va_preservation : forall m t t' ad v V,
   valid_addresses m t ->
-  forall_memory_terms m (valid_addresses m) ->
+  forall_memory m (valid_addresses m) ->
   t --[EF_Write ad v V]--> t' ->
-  forall_memory_terms m[ad <- (v, V)] (valid_addresses m[ad <- (v, V)]).
+  forall_memory m[ad <- (v, V)] (valid_addresses m[ad <- (v, V)]).
 Proof.
   intros. intros ad'. 
-  assert (HasAddress ad t); assert (ad < length m);
-  eauto using step_write_hasad1.
+  assert (ad < length m) by eauto using step_write_hasad1.
   destruct (Nat.eq_dec ad ad'); subst; simpl_array;
   intros ? ?; rewrite set_preserves_length;
   eauto using step_write_hasad2, Nat.lt_lt_succ_r.
@@ -410,49 +262,42 @@ Qed.
 
 Local Corollary mstep_mem_va_preservation : forall m m' t t' eff,
   valid_addresses m t ->
-  forall_memory_terms m (valid_addresses m) ->
+  forall_memory m (valid_addresses m) ->
   m / t ==[eff]==> m' / t' ->
-  forall_memory_terms m' (valid_addresses m').
+  forall_memory m' (valid_addresses m').
 Proof.
   intros. inversion_mstep; trivial;
   eauto using step_alloc_mem_va_preservation, step_write_mem_va_preservation.
 Qed.
 
-(* -------------------------------------------------------------------------- *)
-(* main theorems                                                              *)
-(* -------------------------------------------------------------------------- *)
+(* ------------------------------------------------------------------------- *)
+(* preservation                                                              *)
+(* ------------------------------------------------------------------------- *)
 
-Local Lemma va_spawn_block : forall m t t' block,
-  valid_addresses m t ->
-  t --[EF_Spawn block]--> t' ->
-  valid_addresses m block.
-Proof.
-  intros. induction_step; inversion_va; eauto.
-Qed.
-
-Theorem valid_addresses_preservation1 : forall m m' ths ths' tid eff,
-  forall_memory_terms m (valid_addresses m) ->
+Theorem valid_addresses_term_preservation : forall m m' ths ths' tid eff,
+  forall_memory m (valid_addresses m) ->
   forall_threads ths (valid_addresses m) ->
   m / ths ~~[tid, eff]~~> m' / ths' ->
   forall_threads ths' (valid_addresses m').
 Proof.
   intros. inversion_cstep; intros tid'.
   - destruct (Nat.eq_dec tid tid'); subst; simpl_array;
-    eauto using mstep_va_preservation. intros ? ?.
-    unfold valid_addresses in *. inversion_mstep;
-    try (rewrite add_increments_length || rewrite set_preserves_length);
+    eauto using mstep_va_preservation.
+    intros ? ?. unfold valid_addresses in *.
+    inversion_mstep; eauto;
+    (rewrite add_increments_length || rewrite set_preserves_length);
     eauto using Nat.lt_lt_succ_r.
   - decompose sum (lt_eq_lt_dec tid' (length ths[tid <- t'])); subst;
-    simpl_array; eauto using va_unit, va_spawn_block.
+    simpl_array; eauto using spawn_block_va, va_unit.
     destruct (Nat.eq_dec tid tid'); subst; simpl_array;
     eauto using step_spawn_va_preservation.
 Qed.
 
-Theorem valid_addresses_preservation2 : forall m m' ths ths' tid eff,
+Theorem valid_addresses_memory_preservation : forall m m' ths ths' tid eff,
   forall_threads ths (valid_addresses m) ->
-  forall_memory_terms m (valid_addresses m) ->
+  forall_memory m (valid_addresses m) ->
   m / ths ~~[tid, eff]~~> m' / ths' ->
-  forall_memory_terms m' (valid_addresses m').
+  forall_memory m' (valid_addresses m').
 Proof.
   intros. inversion_cstep; eauto using mstep_mem_va_preservation.
 Qed.
