Contains.v
@@ -59,7 +59,7 @@ Proof.
   intros * Hcon ?. induction Hcon; subst; eauto using Contains.
 Qed.
 
-Lemma step_write_contains_val : forall t t' ad v V,
+Lemma step_write_contains : forall t t' ad v V,
   t --[EF_Write ad v V]--> t' ->
   t contains v.
 Proof.
