HasAddress.v
@@ -1,0 +1,92 @@
+From Coq Require Classical_Prop.
+
+From Elo Require Import Util.
+From Elo Require Import Core.
+
+(* A term has an address <ad> if it contains
+a reference term poiting to <ad>. *)
+Inductive HasAddress (ad : addr) : tm -> Prop :=
+  | hasad_ref : forall T,
+    HasAddress ad <{ &ad :: T }>
+
+  | hasad_new : forall t T,
+    HasAddress ad t ->
+    HasAddress ad <{ new T t }>
+
+  | hasad_load : forall t,
+    HasAddress ad t ->
+    HasAddress ad <{ *t }>
+
+  | hasad_asg1 : forall t1 t2,
+    HasAddress ad t1 ->
+    HasAddress ad <{ t1 = t2 }>
+
+  | hasad_asg2 : forall t1 t2,
+    HasAddress ad t2 ->
+    HasAddress ad <{ t1 = t2 }>
+
+  | hasad_fun : forall t x Tx,
+    HasAddress ad t ->
+    HasAddress ad <{ fn x Tx --> t }>
+
+  | hasad_call1 : forall t1 t2,
+    HasAddress ad t1 ->
+    HasAddress ad <{ call t1 t2 }>
+
+  | hasad_call2 : forall t1 t2,
+    HasAddress ad t2 ->
+    HasAddress ad <{ call t1 t2 }>
+
+  | hasad_seq1 : forall t1 t2,
+    HasAddress ad t1 ->
+    HasAddress ad <{ t1; t2 }>
+
+  | hasad_seq2 : forall t1 t2,
+    HasAddress ad t2 ->
+    HasAddress ad <{ t1; t2 }>
+
+  | hasad_spawn : forall t,
+    HasAddress ad t ->
+    HasAddress ad <{ spawn t }>
+  .
+
+(* ------------------------------------------------------------------------- *)
+(* inversion                                                                 *)
+(* ------------------------------------------------------------------------- *)
+
+Ltac inversion_ha :=
+  match goal with
+  | H : HasAddress _ <{ unit         }> |- _ => inversion H
+  | H : HasAddress _ <{ N _          }> |- _ => inversion H
+  | H : HasAddress _ <{ & _ :: _     }> |- _ => inversion H; subst
+  | H : HasAddress _ <{ new _ _      }> |- _ => inversion H; subst
+  | H : HasAddress _ <{ * _          }> |- _ => inversion H; subst
+  | H : HasAddress _ <{ _ = _        }> |- _ => inversion H; subst
+  | H : HasAddress _ <{ var _        }> |- _ => inversion H
+  | H : HasAddress _ <{ fn _ _ --> _ }> |- _ => inversion H; subst
+  | H : HasAddress _ <{ call _ _     }> |- _ => inversion H; subst
+  | H : HasAddress _ <{ _ ; _        }> |- _ => inversion H; subst
+  | H : HasAddress _ <{ spawn _      }> |- _ => inversion H; subst
+  end.
+
+(* ------------------------------------------------------------------------- *)
+(* properties                                                                *)
+(* ------------------------------------------------------------------------- *)
+
+Lemma step_alloc_hasad : forall t t' ad ad' v V,
+  HasAddress ad v ->
+  t --[EF_Alloc ad' v V]--> t' ->
+  HasAddress ad t.
+Proof. intros. induction_step; eauto using HasAddress. Qed.
+
+Lemma step_write_hasad1 : forall t t' ad v V,
+  t --[EF_Write ad v V]--> t' ->
+  HasAddress ad t.
+Proof. intros. induction_step; eauto using HasAddress. Qed.
+
+Lemma step_write_hasad2 : forall t t' ad ad' v V,
+  HasAddress ad v ->
+  t --[EF_Write ad' v V]--> t' ->
+  HasAddress ad t.
+Proof. intros. induction_step; eauto using HasAddress. Qed.
+
