Util.v
@@ -1,7 +1,7 @@
 From Coq Require Logic.ClassicalFacts.
 From Coq Require Import Logic.Decidable.
 
-(* Miscellaneous Utilities *)
+(* miscellaneous utilities *)
 
 Ltac auto_specialize :=
   match goal with
@@ -11,17 +11,6 @@ Ltac auto_specialize :=
 Ltac inversion_subst_clear H :=
   inversion H; subst; clear H.
 
-(* TODO: classic *)
-Local Lemma destruct_and' : forall a x y,
-  (a -> x /\ y) -> ((a -> x) /\ (a -> y)). 
-Proof.
-  intros * H. split; intros a'; specialize (H a') as [? ?]; trivial.
-Qed.
-
-(* TODO: decompose record ? *)
-Ltac destruct_and H :=
-  eapply destruct_and' in H as [? ?].
-
 Axiom excluded_middle : ClassicalFacts.excluded_middle.
 
 Corollary classic_decidable : forall (P : Prop),
@@ -30,29 +19,3 @@ Proof.
   intros. unfold decidable. eauto using excluded_middle.
 Qed.
 
-(* Unused
-
-Definition memory_has_values (m : mem) :=
-  forall ad, value (getTM m ad).
-
-Theorem memory_has_values_preservation : forall m m' t t' eff,
-  memory_has_values m ->
-  m / t ==[eff]==> m' / t' ->
-  memory_has_values m'.
-Proof.
-  intros. inversion_mstep; trivial.
-  - remember (EF_Alloc _ _) as eff.
-    induction_step; inversion Heqeff; subst; eauto. intros ad.
-    decompose sum (lt_eq_lt_dec ad (length m)); subst.
-    + rewrite (get_add_lt TM_Unit); trivial.
-    + rewrite (get_add_eq TM_Unit); trivial.
-    + rewrite (get_add_gt TM_Unit); eauto using value.
-  - remember (EF_Store _ _) as eff.
-    induction_step; inversion Heqeff; subst; eauto. intros ad'.
-    decompose sum (lt_eq_lt_dec ad' ad); subst.
-    + rewrite (get_set_lt TM_Unit); trivial.
-    + rewrite (get_set_eq TM_Unit); trivial.
-    + rewrite (get_set_gt TM_Unit); trivial.
-Qed.
-
-*)
